Fix tests

src/tls/test/TestDH.fst
@@ -5,6 +5,13 @@ open CoreCrypto
 open CommonDH
 open TLSConstants
 
+val discard: bool -> ST unit
+  (requires (fun _ -> True))
+  (ensures (fun h0 _ h1 -> h0 == h1))
+let discard _ = ()
+let print s = discard (IO.debug_print_string ("TestKS| "^s^"\n"))
+
+
 let main () : ML unit =
   let g = default_group in
   let gx = keygen g in
@@ -13,10 +20,10 @@ let main () : ML unit =
   let gxy  = hex_of_bytes gxy in
   let gxy' = hex_of_bytes gxy' in
   if gxy = gxy' then
-    IO.print_string ("DH exchange test: OK\n")
+    print ("DH exchange test: OK\n")
   else
     begin
-      IO.print_string ("DH exchange test: KO\n");
-      IO.print_string ("Unexpected output: output = " ^ gxy' ^ "\nexpected = " ^ gxy ^ "\n");
+      print ("DH exchange test: KO\n");
+      print ("Unexpected output: output = " ^ gxy' ^ "\nexpected = " ^ gxy ^ "\n");
       failwith "Error!"
     end
